fixing all the proofs in Ext/Expr..
- switching to ExprD1 (easier for the time being)
- writing lemmas to reason about exprD', they are painful.

src/Ext/ExprD1.v
@@ -5,67 +5,11 @@ Require Import MirrorCore.EnvI.
 Require Import MirrorCore.ExprI.
 Require Import MirrorCore.Ext.Types.
 Require Import MirrorCore.Ext.ExprCore.
+Require Import MirrorCore.Ext.ExprT.
+Require Import MirrorCore.Ext.ExprDI.
 
 Set Implicit Arguments.
 Set Strict Implicit.
-
-
-Module Type ExprDenote.
-
-  Parameter typeof : forall (ts : types) (fs : functions ts),
-    env (typD ts) -> tenv typ -> expr -> option typ.
-
-  Parameter exprD : forall (ts : types) (fs : functions ts),
-    env (typD ts) -> env (typD ts) -> expr -> forall t : typ,
-    option (typD ts nil t).
-
-  Section with_envs.
-    Variable ts : types.
-    Variable fs : functions ts.
-    Variable us : env (typD ts).
-
-    Axiom exprD_Var : forall ve v t,
-      exprD fs us ve (Var v) t = lookupAs ve v t.
-
-    Axiom exprD_UVar : forall ve u t,
-      exprD fs us ve (UVar u) t = lookupAs us u t.
-
-    Axiom exprD_Equal : forall ve t l r,
-      exprD fs us ve (Equal t l r) tvProp =
-      match exprD fs us ve l t , exprD fs us ve r t with
-        | Some l , Some r => Some (l = r)
-        | _ , _ => None
-      end.
-
-    Axiom exprD_Not : forall ve p,
-      exprD fs us ve (Not p) tvProp =
-      match exprD fs us ve p tvProp with
-        | Some p => Some (~p)
-        | _ => None
-      end.
-
-    Axiom exprD_Abs : forall ve t u e val,
-      exprD fs us ve (Abs t e) (tvArr t u) = Some val ->
-      forall x, exprD fs us (existT _ t x :: ve) e u = Some (val x).
-
-    Axiom exprD_App : forall ve t e arg,
-      exprD fs us ve (App e arg) t =
-      match typeof fs us (map (@projT1 _ _) ve) e with
-        | Some (tvArr l r) =>
-          match exprD fs us ve e (tvArr l r) , exprD fs us ve arg l , typ_eq_odec r t with
-            | Some f , Some x , Some pf =>
-              match pf in _ = t
-                    return option (typD ts nil t)
-              with
-                | eq_refl => Some (f x)
-              end
-            | _ , _ , _ => None
-          end
-        | _ => None
-      end.
-  End with_envs.
-
-End ExprDenote.
 
 (**
  ** The denotation function with binders must be total because we
@@ -75,21 +19,8 @@ End ExprDenote.
  ** which we can't do until we have the binder.
  **
  **)
-(** There are several potential implementations to this.
- ** (1) exprD : expr -> forall t : typ, option (typD t)
- **   suffers from the problem that since there are now a lot of
- **   [App] you do a lot of duplicate type checking.
- ** (2) exprD_simul : forall e : expr, Checked typD (typeof e)
- **   requires a more complete [typeof] function that checks
- **   all errors eagerly which can cause more work than neccessary.
- ** (3) exprD : expr -> { t : typ & ... -> typD t }
- **   this seems optimal because it avoids dependent types and
- **   will easily allow bouncing between this implementation
- **   and (1) which makes for minimal type checking and no duplicate
- **   work.
- **)
 
-Module EXPR_DENOTE_1 <: ExprDenote.
+Module EXPR_DENOTE_core <: ExprDenote_core.
 
   Section with_envs.
     Variable ts : types.
@@ -140,6 +71,24 @@ Module EXPR_DENOTE_1 <: ExprDenote.
           | Some _ => None
         end
     end.
+
+  Lemma typeof_typeof_expr : forall e ve,
+    typeof_expr (typeof_funcs fs) (typeof_env us) ve e = typeof ve e.
+  Proof.
+    induction e; simpl; intros;
+    repeat match goal with
+             | H : _ |- _ => rewrite H
+           end; auto.
+    { rewrite nth_error_typeof_funcs.
+      destruct (nth_error fs f); auto. }
+    { rewrite nth_error_typeof_env. auto. }
+    { change typ_eqb with (@rel_dec _ (@eq typ) _).
+      destruct (typeof ve e1); auto.
+      destruct (typeof ve e2); auto.
+      consider (t ?[ eq ] t0); auto; intros; subst; auto.
+      destruct (t ?[ eq ] t0); auto. }
+    { destruct (typeof ve e); auto. destruct t; auto. }
+  Qed.
 
   Fixpoint exprD' (var_env : tenv typ) (e : expr) (t : typ) {struct e} :
     option (hlist (typD ts nil) var_env -> typD ts nil t) :=
@@ -198,13 +147,12 @@ Module EXPR_DENOTE_1 <: ExprDenote.
       | App f x =>
         match typeof var_env f with
           | Some (tvArr l r) =>
-            match exprD' var_env f (tvArr l r) , exprD' var_env x l , typ_eq_odec r t with
-              | Some f , Some x , Some pf =>
-                match pf in _ = t
-                      return option (hlist (typD ts nil) var_env -> typD ts nil t)
-                with
-                  | eq_refl => Some (fun v => (f v) (x v))
-                end
+            match exprD' var_env f (tvArr l r)
+                , exprD' var_env x l
+                , typ_cast_typ _ (fun x => x) nil r t
+            with
+              | Some f , Some x , Some cast =>
+                Some (fun v => cast ((f v) (x v)))
               | _ , _ , _ => None
             end
           | _ => None
@@ -222,7 +170,7 @@ Module EXPR_DENOTE_1 <: ExprDenote.
         end
       | Not e =>
         match t as t return option (hlist (typD ts nil) var_env -> typD ts nil t)
- with
+        with
           | tvProp =>
             match exprD' var_env e tvProp with
               | Some P => Some (fun g => not (P g))
@@ -232,784 +180,194 @@ Module EXPR_DENOTE_1 <: ExprDenote.
         end
     end.
 
-  Definition exprD (var_env : env (typD ts)) (e : expr) (t : typ)
-  : option (typD ts nil t) :=
-    let (ts,vs) := split_env var_env in
-    match exprD' ts e t with
-      | None => None
-      | Some f => Some (f vs)
-    end.
-
-  Axiom exprD_Var : forall ve v t,
-      exprD ve (Var v) t = lookupAs ve v t.
-
-    Axiom exprD_UVar : forall ve u t,
-      exprD ve (UVar u) t = lookupAs us u t.
-
-    Axiom exprD_Equal : forall ve t l r,
-      exprD ve (Equal t l r) tvProp =
-      match exprD ve l t , exprD ve r t with
-        | Some l , Some r => Some (l = r)
-        | _ , _ => None
-      end.
-
-    Axiom exprD_Not : forall ve p,
-      exprD ve (Not p) tvProp =
-      match exprD ve p tvProp with
-        | Some p => Some (~p)
-        | _ => None
-      end.
-
-    Axiom exprD_Abs : forall ve t u e val,
-      exprD ve (Abs t e) (tvArr t u) = Some val ->
-      forall x, exprD (existT _ t x :: ve) e u = Some (val x).
-
-    Axiom exprD_App : forall ve t e arg,
-      exprD ve (App e arg) t =
-      match typeof (map (@projT1 _ _) ve) e with
-        | Some (tvArr l r) =>
-          match exprD ve e (tvArr l r) , exprD ve arg l , typ_eq_odec r t with
-            | Some f , Some x , Some pf =>
-              match pf in _ = t
-                    return option (typD ts nil t)
-              with
-                | eq_refl => Some (f x)
-              end
-            | _ , _ , _ => None
-          end
-        | _ => None
-      end.
-  End with_envs.
-End EXPR_DENOTE_1.
-
-Module EXPR_DENOTE_3 <: ExprDenote.
-
-  Section with_envs.
-    Variable ts : types.
-    Variable fs : functions ts.
-    Variable us : env (typD ts).
-
-    Fixpoint typeof (var_env : tenv typ) (e : expr) {struct e} : option typ :=
-    match e with
-      | Var x => nth_error var_env x
-      | UVar x =>
-        match nth_error us x with
-          | None => None
-          | Some tv => Some (projT1 tv)
-        end
-      | Func f ts =>
-        match nth_error fs f with
-          | None => None
-          | Some r =>
-          if EqNat.beq_nat (length ts) (fenv r) then
-            Some (instantiate_typ ts (ftype r))
-          else
-            None
-        end
-      | App e e' =>
-        Monad.bind (typeof var_env e) (fun ft =>
-        Monad.bind (typeof var_env e') (fun xt =>
-        type_of_apply ft xt))
-      | Abs t e =>
-        match typeof (t :: var_env) e with
-          | None => None
-          | Some t' => Some (tvArr t t')
-        end
-      | Equal t e1 e2 => Some tvProp
-      | Not e => Some tvProp
-    end.
-
-  Fixpoint exprD_simul' (var_env : tenv typ) (e : expr) {struct e} :
-    option { t : typ & hlist (typD ts nil) var_env -> typD ts nil t } :=
-    let Z t := hlist (typD ts nil) var_env -> typD ts nil t in
-    match e return option { t : typ & hlist (typD ts nil) var_env -> typD ts nil t } with
-      | Var x =>
-        match nth_error var_env x as pf
-          return pf = nth_error var_env x ->
-                 option { t : typ & hlist (typD ts nil) var_env -> typD ts nil t }
-        with
-          | None => fun _ => None
-          | Some t => fun pf =>
-            Some (existT _ t (fun e => match pf in _ = t''
-                                           return match t'' with
-                                                    | Some t => typD ts nil t
-                                                    | None => unit
-                                                  end -> typD ts nil t with
-                                       | eq_refl => fun x => x
-                                     end (hlist_nth e x)))
-        end eq_refl
-      | UVar x =>
-        match nth_error us x with
-          | None => None
-          | Some (existT t v) => Some (existT Z t (fun _ => v))
-        end
-      | Func f ts' =>
-        match nth_error fs f with
-          | None => None
-          | Some f =>
-            match type_apply _ _ ts' _ _ f.(fdenote) with
-              | None => None
-              | Some v =>
-                Some (existT Z (instantiate_typ ts' (ftype f)) (fun _ => v))
-            end
-        end
-      | Abs t' e =>
-        match exprD_simul' (t' :: var_env) e with
-          | None => None
-          | Some (existT t v) =>
-            Some (existT (fun t => hlist (typD ts nil) var_env -> typD ts nil t) (tvArr t' t) (fun g x => v (Hcons x g)))
-        end
-      | App f x =>
-        match exprD_simul' var_env f with
-          | None => None
-          | Some (existT (tvArr l r) f) =>
-            match exprD' var_env x l with
-              | None => None
-              | Some x => Some (existT (fun t => hlist (typD ts nil) var_env -> typD ts nil t) r (fun v => (f v) (x v)))
-            end
-          | _ => None
-        end
-      | Equal t e1 e2 =>
-        match exprD' var_env e1 t , exprD' var_env e2 t with
-          | Some v1, Some v2 =>
-            Some (existT Z tvProp (fun v => @eq _ (v1 v) (v2 v)))
-          | _ , _ => None
-        end
-      | Not e =>
-        match exprD' var_env e tvProp with
-          | None => None
-          | Some P => Some (existT Z tvProp (fun v => not (P v)))
-        end
-    end
-  with exprD' (var_env : tenv typ) (e : expr) (t : typ) {struct e} :
-    option (hlist (typD ts nil) var_env -> typD ts nil t) :=
-    match e with
-      | Var x =>
-        match nth_error var_env x as z
-          return z = nth_error var_env x ->
-                 option (hlist (typD ts nil) var_env -> typD ts nil t)
-        with
-          | None => fun _ => None
-          | Some t' => fun pf =>
-            match typ_cast_typ ts (fun x => x) _ t' t with
-              | Some f =>
-                Some (fun e => match pf in _ = t''
-                                     return match t'' with
-                                              | Some t => typD ts nil t
-                                              | None => unit
-                                            end -> typD ts nil t with
-                                 | eq_refl => fun x => f x
-                               end (hlist_nth e x))
-              | None => None
-            end
-        end eq_refl
-      | UVar x =>
-        match lookupAs us x t with
-          | None => None
-          | Some v => Some (fun _ => v)
-        end
-      | Func f ts' =>
-        match nth_error fs f with
-          | None => None
-          | Some f =>
-            match type_apply _ _ ts' _ _ f.(fdenote) with
-              | None => None
-              | Some t' =>
-                match @typ_cast_val _ _ (instantiate_typ ts' (ftype f)) t t' with
-                  | Some v => Some (fun _ => v)
-                  | None => None
-                end
-            end
-        end
-      | Abs t' e =>
-        match t as t return option (hlist (typD ts nil) var_env -> typD ts nil t)
-        with
-          | tvArr lt rt =>
-            match typ_cast_typ ts (fun x => x) nil lt t' with
-              | None => None
-              | Some cast =>
-                match @exprD' (lt :: var_env) e rt with
-                  | None => None
-                  | Some a => Some (fun x y => a (Hcons y x))
-                end
-            end
-          | _ => None
-        end
-      | App f x =>
-        match exprD_simul' var_env f with
-          | Some (existT (tvArr l r) f) =>
-            match exprD' var_env x l with
-              | None => None
-              | Some x =>
-                match typ_cast_typ ts (fun x => x) _ r t with
-                  | None => None
-                  | Some cast => Some (fun v => cast ((f v) (x v)))
-                end
-            end
-          | _ => None
-        end
-      | Not e =>
-        match t as t
-              return option (hlist (typD ts nil) var_env -> typD ts nil t)
-        with
-          | tvProp => match exprD' var_env e tvProp with
-                        | None => None
-                        | Some P => Some (fun v => not (P v))
-                      end
-          | _ => None
-        end
-      | Equal t' e1 e2 =>
-        match t as t return option (hlist (typD ts nil) var_env -> typD ts nil t) with
-          | tvProp =>
-            match exprD' var_env e1 t' , exprD' var_env e2 t' with
-              | Some l , Some r =>
-                Some (fun g => (l g) = (r g))
-              (* equal (type := typeFor (typD := typD ts) nil t') *)
-              | _ , _ => None
-            end
-          | _ => None
-        end
-    end.
-
-  Definition exprD (var_env : env (typD ts)) (e : expr) (t : typ)
-  : option (typD ts nil t) :=
-    let (ts,vs) := split_env var_env in
-    match exprD' ts e t with
-      | None => None
-      | Some f => Some (f vs)
-    end.
-
-Require Import ExtLib.Tactics.Injection.
-  Require Import ExtLib.Tactics.EqDep.
-  Require Import ExtLib.Data.ListNth.
-
-
-    Theorem split_env_nth_error : forall ve v tv,
-      nth_error ve v = Some tv <->
-      match nth_error (projT1 (split_env ve)) v as t
-      return match t with
-               | Some v => typD ts nil v
-               | None => unit
-             end -> Prop
-      with
-        | None => fun _ => False
-        | Some v => fun res => tv = existT _ v res
-      end (hlist_nth (projT2 (split_env ve)) v).
+    Theorem exprD'_Abs : forall ve t e u,
+       exprD' ve (Abs t e) u =
+       match u as u return option (hlist (typD ts nil) ve -> typD ts nil u) with
+         | tvArr l r =>
+           match typ_cast_typ _ (fun x => x) _ l t
+               , exprD' (t :: ve) e r
+           with
+             | Some cast , Some f =>
+               Some (fun g => fun x => f (Hcons (F := typD ts nil) (cast x) g))
+             | _ , _ => None
+           end
+         | _ => None
+       end.
     Proof.
-      induction ve; simpl; intros.
-      { destruct v; simpl in *; intuition; inversion H. }
-      { destruct v; simpl in *.
-        { intuition.
-          { inversion H; subst. destruct tv; reflexivity. }
-          { subst. destruct a. reflexivity. } }
-        { eapply IHve. } }
+      simpl. destruct u; auto.
+      remember (typ_cast_typ ts (fun x : Type => x) nil u1 t).
+      destruct o; auto.
+      symmetry in Heqo.
+      generalize (typ_cast_typ_eq ts (fun x => x) nil u1 t Heqo); intros; subst.
+      rewrite typ_cast_typ_refl in Heqo.
+      Require Import ExtLib.Tactics.Injection.
+      inv_all; subst. reflexivity.
     Qed.
 
-  Theorem exprD_Var : forall ve v t,
-    exprD ve (Var v) t = lookupAs ve v t.
-  Proof.
-    unfold exprD; simpl; intros.
-    consider (split_env ve); intros.
-    unfold lookupAs.
-    generalize (split_env_nth_error ve v).
-    consider (nth_error ve v).
-    { intros. destruct (H1 s); clear H1. clear H3. specialize (H2 eq_refl).
-      rewrite H in *. simpl in *.
-      destruct s; simpl in *.
-      revert H2.
-      change (
-          let f' e0 := hlist_nth e0 v in
-          match
-            nth_error x v as t1
-            return
-            (match t1 with
-               | Some v0 => typD ts nil v0
-               | None => unit
-             end -> Prop)
-          with
-            | Some v0 =>
-              fun res : typD ts nil v0 =>
-                existT (typD ts nil) x0 t0 = existT (typD ts nil) v0 res
-            | None => fun _ : unit => False
-          end (f' h) ->
-          match
-            match
-              nth_error x v as z
-              return
-              (z = nth_error x v ->
-               option (hlist (typD ts nil) x -> typD ts nil t))
-            with
-              | Some t' =>
-                fun pf : Some t' = nth_error x v =>
-                  match typ_cast_typ ts (fun x1 : Type => x1) nil t' t with
-                    | Some f =>
-                      Some
-                        (fun e0 : hlist (typD ts nil) x =>
-                           match
-                             pf in (_ = t'')
-                             return
-                             (match t'' with
-                                | Some t1 => typD ts nil t1
-                                | None => unit
-                              end -> typD ts nil t)
-                           with
-                             | eq_refl => fun x1 : typD ts nil t' => f x1
-                           end (f' e0))
-                    | None => None
-                  end
-              | None => fun _ : None = nth_error x v => None
-            end eq_refl
-          with
-            | Some f => Some (f h)
+    Theorem exprD'_Var : forall ve v t,
+      exprD' ve (Var v) t =
+      match nth_error ve v as z
+            return z = nth_error ve v ->
+                   option (hlist (typD ts nil) ve -> typD ts nil t)
+      with
+        | Some z => fun pf =>
+          match typ_cast_typ _ (fun x => x) _ z t with
+            | Some cast =>
+              Some (fun e => match pf in _ = t''
+                                   return match t'' with
+                                            | Some t => typD ts nil t
+                                            | None => unit
+                                          end -> typD ts nil t with
+                               | eq_refl => fun x => cast x
+                             end (hlist_nth e v))
             | None => None
-          end =
-          match typ_cast_typ ts (fun x1 : Type => x1) nil x0 t with
-            | Some f => Some (f t0)
-            | None => None
-          end).
+          end
+        | None => fun _ => None
+      end eq_refl.
+    Proof.
+      simpl; intros.
       match goal with
         | |- context [ @eq_refl ?X ?Y ] =>
-          generalize dependent (@eq_refl X Y)
+          generalize (@eq_refl X Y)
       end.
-      pattern (nth_error x v) at 1 5.
-      destruct (nth_error x v).
-      { intro.
-        assert (nth_error x v = Some x0).
-        { cutrewrite (x = projT1 (split_env ve)).
-          rewrite split_env_projT1.
-          erewrite map_nth_error. 2: eassumption. reflexivity.
-          rewrite H. reflexivity. }
-        { assert (x0 = t1).
-          { rewrite H1 in e. inv_all; auto. }
-          subst. destruct (typ_cast_typ ts (fun x => x) nil t1 t); auto.
-          { intros. f_equal.
-            subst f'. simpl in *. generalize dependent (hlist_nth h v).
-            generalize dependent (nth_error x v).
-            intros; subst.
-            inv_all. f_equal; auto. } } }
-      { simpl. intro. generalize dependent (hlist_nth h v).
-        rewrite <- e. intuition. } }
-    { intro.
-      assert (nth_error x v = None).
-      { cutrewrite (x = projT1 (split_env ve)).
-        rewrite split_env_projT1.
-        rewrite nth_error_map.
-        rewrite H0. reflexivity.
-        rewrite H. reflexivity. }
-      { match goal with
-          | |- context [ @eq_refl ?X ?Y ] =>
-            generalize dependent (@eq_refl X Y)
-        end.
-        rewrite H; simpl. intros. clear H2.
-        change (
-            let f t' := fun pf : Some t' = nth_error x v =>
-                    match typ_cast_typ ts (fun x0 : Type => x0) nil t' t with
-                      | Some f =>
-                        Some
-                          (fun e0 : hlist (typD ts nil) x =>
-                             match
-                               pf in (_ = t'')
-                               return
-                               (match t'' with
-                                  | Some t0 => typD ts nil t0
-                                  | None => unit
-                                end -> typD ts nil t)
-                             with
-                               | eq_refl => fun x0 : typD ts nil t' => f x0
-                             end (hlist_nth e0 v))
-                      | None => None
-                    end in
-            match
+      change (let zzz := fun e0 => hlist_nth e0 v in
+              forall e : nth_error ve v = nth_error ve v,
+   match
+     nth_error ve v as z
+     return
+       (z = nth_error ve v ->
+        option (hlist (typD ts nil) ve -> typD ts nil t))
+   with
+   | Some t' =>
+       fun pf : Some t' = nth_error ve v =>
+       match typ_cast_typ ts (fun x : Type => x) nil t' t with
+       | Some f =>
+           Some
+             (fun e0 : hlist (typD ts nil) ve =>
               match
-                nth_error x v as z
+                pf in (_ = t'')
                 return
-                (z = nth_error x v ->
-                 option (hlist (typD ts nil) x -> typD ts nil t))
+                  (match t'' with
+                   | Some t0 => typD ts nil t0
+                   | None => unit
+                   end -> typD ts nil t)
               with
-                | Some t' => f t'
-                | None => fun _ : None = nth_error x v => None
-              end e
-            with
-              | Some f => Some (f h)
-              | None => None
-            end = None
-          ).
-        intro. clearbody f.
-        revert e.
-        pattern (nth_error x v) at 1 3.
-        rewrite H1. reflexivity. } }
-  Qed.
-
-  Theorem exprD_UVar : forall ve u t,
-    exprD ve (UVar u) t = lookupAs us u t.
-  Proof.
-    unfold exprD. intros.
-    destruct (split_env ve); simpl.
-    destruct (lookupAs us u t); auto.
-  Qed.
-
-  Theorem exprD_Equal : forall ve t l r,
-    exprD ve (Equal t l r) tvProp =
-    match exprD ve l t , exprD ve r t with
-      | Some l , Some r => Some (l = r)
-      | _ , _ => None
-    end.
-  Proof.
-    unfold exprD; intros.
-    destruct (split_env ve); simpl.
-    destruct (exprD' x l t); destruct (exprD' x r t); auto.
-  Qed.
-
-  Theorem exprD_Not : forall ve p,
-    exprD ve (Not p) tvProp =
-    match exprD ve p tvProp with
-      | Some p => Some (~p)
-      | _ => None
-    end.
-  Proof.
-    unfold exprD; intros.
-    destruct (split_env ve); simpl.
-    destruct (exprD' x p tvProp); auto.
-  Qed.
-
-   Theorem exprD_Abs : forall ve t u e val,
-      exprD ve (Abs t e) (tvArr t u) = Some val ->
-      forall x, exprD (existT _ t x :: ve) e u = Some (val x).
-   Proof.
-    unfold exprD. intros.
-    change (split_env (existT (typD ts nil) t x :: ve))
-      with (split_env ((existT (typD ts nil) t x :: nil) ++ ve)).
-    rewrite split_env_app.
-    destruct (split_env ve). simpl in *.
-    rewrite typ_cast_typ_refl in *.
-    destruct (exprD' (t :: x0) e u); intuition (try congruence).
-    inv_all; subst. reflexivity.
-  Qed.
-
-   Theorem exprD_App : forall ve t e arg,
-      exprD ve (App e arg) t =
-      match typeof (map (@projT1 _ _) ve) e with
-        | Some (tvArr l r) =>
-          match exprD ve e (tvArr l r) , exprD ve arg l , typ_eq_odec r t with
-            | Some f , Some x , Some pf =>
-              match pf in _ = t
-                    return option (typD ts nil t)
+              | eq_refl => fun x : typD ts nil t' => f x
+              end (zzz e0))
+       | None => None
+       end
+   | None => fun _ : None = nth_error ve v => None
+   end e =
+   match
+     nth_error ve v as z
+     return
+       (z = nth_error ve v ->
+        option (hlist (typD ts nil) ve -> typD ts nil t))
+   with
+   | Some z =>
+       fun pf : Some z = nth_error ve v =>
+       match typ_cast_typ ts (fun x : Type => x) nil z t with
+       | Some cast =>
+           Some
+             (fun e0 : hlist (typD ts nil) ve =>
+              match
+                pf in (_ = t'')
+                return
+                  (match t'' with
+                   | Some t0 => typD ts nil t0
+                   | None => unit
+                   end -> typD ts nil t)
               with
-                | eq_refl => Some (f x)
+              | eq_refl => fun x : typD ts nil z => cast x
+              end (zzz e0))
+       | None => None
+       end
+   | None => fun _ : None = nth_error ve v => None
+   end e).
+      intro.
+      clearbody zzz. revert zzz.
+      destruct (nth_error ve v); auto.
+    Qed.
+
+    Theorem exprD'_UVar : forall ve u t,
+      exprD' ve (UVar u) t =
+      match lookupAs us u t with
+        | Some z => Some (fun _ => z)
+        | None => None
+      end.
+    Proof.
+      reflexivity.
+    Qed.
+
+    Theorem exprD'_Func : forall ve f ts t,
+      exprD' ve (Func f ts) t =
+      match nth_error fs f with
+        | None => None
+        | Some f =>
+          match type_apply _ _ ts _ _ f.(fdenote) with
+            | None => None
+            | Some t' =>
+              match @typ_cast_typ _ (fun x => x) _ (instantiate_typ ts (ftype f)) t with
+                | None => None
+                | Some cast => Some (fun _ => cast t')
               end
+          end
+      end.
+    Proof.
+      simpl; intros.
+      destruct (nth_error fs f); auto.
+      destruct (type_apply ts (fenv f0) ts0 nil (ftype f0) (fdenote f0)); auto.
+      unfold typ_cast_val.
+      destruct (typ_cast_typ ts (fun x : Type => x) nil
+         (instantiate_typ ts0 (ftype f0)) t); auto.
+    Qed.
+
+    Theorem exprD'_Equal : forall ve t l r t',
+      exprD' ve (Equal t l r) t' =
+      match t' as t' return option (hlist (typD ts nil) ve -> typD ts nil t') with
+        | tvProp =>
+          match exprD' ve l t , exprD' ve r t with
+            | Some l , Some r => Some (fun g => l g = r g)
+            | _ , _ => None
+          end
+        | _ => None
+      end.
+    Proof.
+      reflexivity.
+    Qed.
+
+    Theorem exprD'_Not : forall ve p t',
+      exprD' ve (Not p) t' =
+      match t' as t' return option (hlist (typD ts nil) ve -> typD ts nil t') with
+        | tvProp =>
+          match exprD' ve p tvProp with
+            | Some p => Some (fun g => not (p g))
+            | _ => None
+          end
+        | _ => None
+      end.
+    Proof. reflexivity. Qed.
+
+    Theorem exprD'_App : forall ve t e arg,
+      exprD' ve (App e arg) t =
+      match typeof_expr (typeof_funcs fs) (typeof_env us) ve e with
+        | Some (tvArr l r) =>
+          match exprD' ve e (tvArr l r)
+              , exprD' ve arg l
+              , typ_cast_typ _ (fun x => x) _ r t
+          with
+            | Some f , Some x , Some cast =>
+              Some (fun g => cast ((f g) (x g)))
             | _ , _ , _ => None
           end
         | _ => None
       end.
-   Proof.
-     unfold exprD; intros.
-    destruct (split_env ve); simpl.
-    rewrite <- split_env_projT1.
-   Admitted.
+    Proof.
+      simpl; intros.
+      rewrite typeof_typeof_expr. reflexivity.
+    Qed.
 
   End with_envs.
-End EXPR_DENOTE_3.
+End EXPR_DENOTE_core.
 
-Module EXPR_DENOTE_2 <: ExprDenote.
-  Require Import ExtLib.Data.Checked.
-
-  Section with_envs.
-    Variable ts : types.
-    Variable fs : functions ts.
-    Variable us : env (typD ts).
-
-    Definition todo : forall T : Type, T. Admitted.
-
-
-    Definition rapply te (ft xt : typ) :
-    Checked (fun t => typD ts te ft -> typD ts te xt -> typD ts te t)
-            (type_of_apply ft xt) :=
-    match ft as ft
-          return Checked (fun t => typD ts te ft -> typD ts te xt -> typD ts te t)
-                         (type_of_apply ft xt)
-    with
-      | tvArr l r =>
-        match typ_eqb l xt as e
-              return typ_eqb l xt = e ->
-                     Checked (fun t => typD ts te (tvArr l r) -> typD ts te xt -> typD ts te t)
-                             (if e then Some r else None)
-        with
-          | true => fun pf =>
-            @Success _ _ _  (fun f x => f (match eq_sym (typ_eqb_true _ _ pf) in _ = t
-                                                 return typD ts te t
-                                           with
-                                             | eq_refl => x
-                                           end))
-          | false => fun _ => Failure _
-        end eq_refl
-      | _ => Failure _
-    end.
-
-Fixpoint typeof (var_env : tenv typ) (e : expr) {struct e} : option typ :=
-    match e with
-      | Var x => nth_error var_env x
-      | UVar x =>
-        match nth_error us x with
-          | None => None
-          | Some tv => Some (projT1 tv)
-        end
-      | Func f ts =>
-        match nth_error fs f with
-          | None => None
-          | Some r =>
-          if EqNat.beq_nat (length ts) (fenv r) then
-            Some (instantiate_typ ts (ftype r))
-          else
-            None
-        end
-      | App e e' =>
-        Monad.bind (typeof var_env e) (fun ft =>
-        Monad.bind (typeof var_env e') (fun xt =>
-        type_of_apply ft xt))
-      | Abs t e =>
-        match typeof (t :: var_env) e with
-          | None => None
-          | Some t' => Some (tvArr t t')
-        end
-      | Equal t e1 e2 =>
-        match typeof var_env e1 with
-          | None => None
-          | Some t' => match typeof var_env e2 with
-                         | None => None
-                         | Some t'' => if t ?[ eq ] t' then
-                                         if t' ?[ eq ] t'' then Some tvProp
-                                         else None
-                                       else None
-                       end
-        end
-      | Not e =>
-        match typeof var_env e with
-          | None => None
-          | Some tvProp => Some tvProp
-          | Some _ => None
-        end
-    end.
-
-  Fixpoint exprD_simul' (var_env : tenv typ) (e : expr) {struct e} :
-    Checked (fun t => hlist (typD ts nil) var_env -> typD ts nil t)
-            (typeof var_env e) :=
-    let Z := (fun t => hlist (typD ts nil) var_env -> typD ts nil t) in
-    match e as e
-      return Checked Z (typeof var_env e)
-    with
-      | Var x =>
-        match nth_error var_env x as z
-          return z = nth_error var_env x -> Checked Z z
-        with
-          | None => fun _ => Failure _
-          | Some t => fun pf =>
-            @Success _ Z
-                     t (fun e => match pf in _ = t''
-                                     return match t'' with
-                                              | Some t => typD ts nil t
-                                              | None => unit
-                                            end -> typD ts nil t with
-                                 | eq_refl => fun x => x
-                               end (hlist_nth e x))
-        end eq_refl
-      | UVar x =>
-        match nth_error us x as tv
-              return Checked (fun t : typ => hlist (typD ts nil) var_env -> typD ts nil t)
-                             (match tv with
-                                | None => None
-                                | Some tv => Some (projT1 tv)
-                              end)
-        with
-          | None => Failure _
-          | Some t =>
-            @Success _ Z
-                     (projT1 t) (fun _ : hlist (typD ts nil) var_env => projT2 t)
-        end
-      | Func f ts' => todo _
-(*
-        match nth_error funcs f as ft
-              return Checked (fun t : typ => hlist (typD ts nil) var_env -> typD ts nil t)
-                             (match ft with
-                                | None => None
-                                | Some r => Some (instantiate_typ ts' (ftype r))
-                              end)
-        with
-          | None => Failure _
-          | Some f =>
-            match type_apply _ _ ts' _ _ f.(fdenote) with
-              | None => Failure _
-              | Some v =>
-                @Success _ Z
-                         (instantiate_typ ts' (ftype f)) (fun _ => v)
-            end
-        end *)
-      | Abs t' e =>
-        match @exprD_simul' (t' :: var_env) e in Checked _ tc
-              return Checked Z
-                             (match tc with
-                                | None => None
-                                | Some t'' => Some (tvArr t' t'')
-                              end)
-        with
-          | Failure => Failure _
-          | Success t v => @Success _ (fun t => hlist (typD ts nil) var_env ->
-                                       typD ts nil t)
-                                    (tvArr t' t)
-                                    (fun g => fun x => v (Hcons x g))
-        end
-      | App f x =>
-        match exprD_simul' var_env f in Checked _ tc
-              return Checked Z
-                             (match tc with
-                                | None => None
-                                | Some tf => match typeof var_env x with
-                                                | None => None
-                                                | Some tx => type_of_apply tf tx
-                                             end
-                              end)
-        with
-          | Failure => Failure _
-          | Success tf f =>
-            match exprD_simul' var_env x in Checked _ tc
-                  return Checked Z
-                                 (match tc with
-                                    | None => None
-                                    | Some tx => type_of_apply tf tx
-                                  end)
-            with
-              | Failure => Failure _
-              | Success tx x =>
-                match rapply nil tf tx with
-                  | Failure => Failure _
-                  | Success t ap =>
-                    @Success _ Z
-                             t (fun v => ap (f v) (x v))
-                end
-            end
-        end
-      | Equal t e1 e2 =>
-        match exprD_simul' var_env e1 in Checked _ tc
-              return Checked Z
-                             (match tc with
-                                | None => None
-                                | Some t' =>
-                                  match typeof var_env e2 with
-                                    | None => None
-                                    | Some t'' => if t ?[ eq ] t' then
-                                                    if t' ?[ eq ] t'' then Some tvProp
-                                                    else None
-                                                  else None
-                                  end
-                              end)
-        with
-          | Failure => Failure _
-          | Success t1 v1 =>
-            match exprD_simul' var_env e2 in Checked _ tc
-                  return Checked Z
-                                 (match tc with
-                                      | None => None
-                                      | Some t'' => if t ?[ eq ] t1 then
-                                                      if t1 ?[ eq ] t'' then Some tvProp
-                                                      else None
-                                                    else None
-                                  end)
-            with
-              | Failure => Failure _
-              | Success t2 v2 =>
-                match t ?[ eq ] t1 as res
-                      return Checked Z
-                                 (if res then
-                                    if t1 ?[ eq ] t2 then Some tvProp
-                                    else None
-                                  else None)
-                with
-                  | false => Failure _
-                  | true =>
-                    match t1 ?[ eq ] t2 as res
-                          return t1 ?[ eq ] t2 = res ->
-                                 Checked Z
-                                         (if res then Some tvProp else None)
-                    with
-                      | false => fun _ => Failure _
-                      | true => fun pf =>
-                                  match ((proj1 (rel_dec_correct _ _)) pf) in _ = t
-                                        return (hlist (typD ts nil) var_env -> typD ts nil t) ->
-                                               Checked Z
-                                                       (Some tvProp)
-                                  with
-                                    | eq_refl => fun v2 =>
-                                      @Success _ Z
-                                               tvProp (fun v => @eq _ (v1 v) (v2 v))
-                                  end v2
-                    end eq_refl
-                end
-            end
-        end
-      | Not e =>
-        match exprD_simul' var_env e in Checked _ tc
-              return Checked Z
-                             match tc with
-                               | Some tvProp => Some tvProp
-                               | _ => None
-                             end
-        with
-          | Failure => Failure _
-          | Success tvProp P =>
-            @Success _ Z
-                     tvProp (fun g => not (P g))
-          | Success _ _ => Failure _
-        end
-    end.
-
-  Definition exprD (var_env : env (typD ts)) (e : expr) (t : typ)
-  : option (typD ts nil t) :=
-    let (ts',vs) := split_env var_env in
-    match exprD_simul' ts' e with
-      | Success t' v =>
-        @typ_cast_val ts nil  t' t (v vs)
-      | Failure => None
-    end.
-
-
-    Axiom exprD_Var : forall ve v t,
-      exprD ve (Var v) t = lookupAs ve v t.
-
-    Axiom exprD_UVar : forall ve u t,
-      exprD ve (UVar u) t = lookupAs us u t.
-
-    Axiom exprD_Equal : forall ve t l r,
-      exprD ve (Equal t l r) tvProp =
-      match exprD ve l t , exprD ve r t with
-        | Some l , Some r => Some (l = r)
-        | _ , _ => None
-      end.
-
-    Axiom exprD_Not : forall ve p,
-      exprD ve (Not p) tvProp =
-      match exprD ve p tvProp with
-        | Some p => Some (~p)
-        | _ => None
-      end.
-
-    Axiom exprD_Abs : forall ve t u e val,
-      exprD ve (Abs t e) (tvArr t u) = Some val ->
-      forall x, exprD (existT _ t x :: ve) e u = Some (val x).
-
-    Axiom exprD_App : forall ve t e arg,
-      exprD ve (App e arg) t =
-      match typeof (map (@projT1 _ _) ve) e with
-        | Some (tvArr l r) =>
-          match exprD ve e (tvArr l r) , exprD ve arg l , typ_eq_odec r t with
-            | Some f , Some x , Some pf =>
-              match pf in _ = t
-                    return option (typD ts nil t)
-              with
-                | eq_refl => Some (f x)
-              end
-            | _ , _ , _ => None
-          end
-        | _ => None
-      end.
-
-  End with_envs.
-End EXPR_DENOTE_2.
+Module EXPR_DENOTE := Build_ExprDenote EXPR_DENOTE_core.
